Initial commit (still tweaking the rules)

syntax.sig
@@ -2,6 +2,7 @@ nat  : Type
 Tm(VarTm) : Type
 PTag : Type
 TTag : Type
+bool : Type
 
 TPi : TTag
 TSig : TTag
@@ -14,3 +15,6 @@ Proj : PTag -> Tm -> Tm
 TBind : TTag -> Tm -> (bind Tm in Tm) -> Tm
 Bot : Tm
 Univ : nat -> Tm
+Bool : Tm
+BVal : bool -> Tm
+If : Tm -> Tm -> Tm -> Tm
